Update duplicate proofs to work with lists of type T.

CrDsl.v
@@ -8,6 +8,7 @@ Require Import Strings.String.
 From MyProject Require Export CrIdentifiers.
 From MyProject Require Export CrTransformer.
 From MyProject Require Export ListUtils.
+Require Import Coq.Bool.Bool.
 
 (* A Module has a module name and either a parser or transformer definition *)
 Inductive Module : Type := 
@@ -34,32 +35,49 @@ Inductive CaracaraProgram : Type :=
 Definition check_for_duplicate_identifiers (program : CaracaraProgram) : bool :=
   match program with
   | CaracaraProgramDef p h s m f c cc _ _ =>
-      has_duplicates (fun x y =>
-            match x, y with
-            | ParserStateCtr xid, ParserStateCtr yid => Nat.eqb xid yid
-            end) p ||
-      has_duplicates (fun x y =>
-            match x, y with
-            | HeaderCtr xid, HeaderCtr yid => Nat.eqb xid yid
-            end) h ||
-      has_duplicates (fun x y =>
-            match x, y with
-            | StateVarCtr xid, StateVarCtr yid => Nat.eqb xid yid
-            end) s ||
-      has_duplicates (fun x y =>
-            match x, y with
-            | ModuleNameCtr xid, ModuleNameCtr yid => Nat.eqb xid yid
-            end) m ||
-      has_duplicates (fun x y =>
-            match x, y with
-            | FunctionNameCtr xid, FunctionNameCtr yid => Nat.eqb xid yid
-            end) f ||
-      has_duplicates (fun x y =>
-            match x, y with
-            | ConnectionNameCtr xid, ConnectionNameCtr yid => Nat.eqb xid yid
-            end) c ||
-      has_duplicates (fun x y =>
-            match x, y with
-            | CtrlPlaneConfigNameCtr xid, CtrlPlaneConfigNameCtr yid => Nat.eqb xid yid
-            end) cc
+      has_duplicates parser_state_equal p ||
+      has_duplicates header_equal h ||
+      has_duplicates state_var_equal s ||
+      has_duplicates module_name_equal m ||
+      has_duplicates function_name_equal f ||
+      has_duplicates connection_name_equal c ||
+      has_duplicates ctrl_plane_config_name_equal cc
   end.
+
+  (* No duplicates in Caracara Program *)
+  Definition CaracaraNoDup (p : CaracaraProgram) : Prop :=
+  match p with
+  | CaracaraProgramDef ps hs svs mns fns cns cpns _ _  =>
+      NoDup ps /\ NoDup hs /\ NoDup svs /\ NoDup mns /\
+      NoDup fns /\ NoDup cns /\ NoDup cpns
+  end.
+
+  (* Check if any of the identifier lists in the CR program has duplicates.
+     Use the check_for_duplicate_identifiers function above.
+     If it returns false, it implies there are no duplicates. *)
+Lemma check_for_duplicates_in_cr_program :
+    forall (p : CaracaraProgram),
+      check_for_duplicate_identifiers (p) = false ->
+        CaracaraNoDup p.
+Proof.
+    intros p.
+    intros H.
+    destruct p.
+    unfold CaracaraNoDup.
+    simpl in H.
+    apply orb_false_iff in H as [H' H7].
+    apply orb_false_iff in H' as [H'' H6].
+    apply orb_false_iff in H'' as [H''' H5].
+    apply orb_false_iff in H''' as [H'''' H4].
+    apply orb_false_iff in H'''' as [H''''' H3].
+    apply orb_false_iff in H''''' as [H1 H2].
+    (* Now H'''''' is the first, H2 is the second, ..., H7 is the last *)
+    repeat split.
+    - apply has_duplicates_correct with (eqb := parser_state_equal). apply H1.
+    - apply has_duplicates_correct with (eqb := header_equal). apply H2.
+    - apply has_duplicates_correct with (eqb := state_var_equal). apply H3.
+    - apply has_duplicates_correct with (eqb := module_name_equal). apply H4.
+    - apply has_duplicates_correct with (eqb := function_name_equal). apply H5.
+    - apply has_duplicates_correct with (eqb := connection_name_equal). apply H6.
+    - apply has_duplicates_correct with (eqb := ctrl_plane_config_name_equal). apply H7.
+Qed.
