CrIdentifiers.v
@@ -13,3 +13,45 @@ Inductive ModuleName : Type := ModuleNameCtr (uid : nat).
 Inductive FunctionName : Type := FunctionNameCtr (uid : nat).
 Inductive ConnectionName : Type := ConnectionNameCtr (uid : nat).
 Inductive CtrlPlaneConfigName : Type := CtrlPlaneConfigNameCtr (uid : nat).
+
+(* Equality check functions for the identifiers above *)
+Definition parser_state_equal (p1 p2 : ParserState) :=
+    match p1, p2 with
+            | ParserStateCtr xid, ParserStateCtr yid => Nat.eqb xid yid
+    end.
+
+(* Do the same thing as parser_state_equal for Header *)
+Definition header_equal (h1 h2 : Header) :=
+    match h1, h2 with
+            | HeaderCtr xid, HeaderCtr yid => Nat.eqb xid yid
+    end.
+
+(* Do the same thing as parser_state_equal for StateVar *)
+Definition state_var_equal (sv1 sv2 : StateVar) :=
+    match sv1, sv2 with
+            | StateVarCtr xid, StateVarCtr yid => Nat.eqb xid yid
+    end.
+
+(* Do the same thing as parser_state_equal for ModuleName *)
+Definition module_name_equal (m1 m2 : ModuleName) :=
+    match m1, m2 with
+            | ModuleNameCtr xid, ModuleNameCtr yid => Nat.eqb xid yid
+    end.
+
+(* Do the same thing as parser_state_equal for FunctionName *)
+Definition function_name_equal (f1 f2 : FunctionName) :=
+    match f1, f2 with
+            | FunctionNameCtr xid, FunctionNameCtr yid => Nat.eqb xid yid
+    end.
+
+(* Do the same thing as parser_state_equal for ConnectionName *)
+Definition connection_name_equal (c1 c2 : ConnectionName) :=
+    match c1, c2 with
+            | ConnectionNameCtr xid, ConnectionNameCtr yid => Nat.eqb xid yid
+    end.
+
+(* Do the same thing as parser_state_equal for CtrlPlaneConfigName *)
+Definition ctrl_plane_config_name_equal (cc1 cc2 : CtrlPlaneConfigName) :=
+    match cc1, cc2 with
+            | CtrlPlaneConfigNameCtr xid, CtrlPlaneConfigNameCtr yid => Nat.eqb xid yid
+    end.
